TinyBCT/Tests/Tests.cs
@@ -1917,19 +1917,19 @@ public class TestsManu : TestsBase
 
     [TestMethod]
     [TestCategory("Manu")]
-    [Ignore] // Remove (or change test) once bug related to ref keyword is fixed
+    // Remove (or change test) once bug related to ref keyword is fixed
     public void RefKeyword1()
     {
-        var corralResult = CorralTestHelper("RefKeyword", @"Test.RefKeyword.Main", 10);
+        var corralResult = CorralTestHelper("RefKeyword", @"Test.RefKeyword.Main", 10, additionalTinyBCTOptions: "/NewAddrModelling=true");
         Assert.IsTrue(corralResult.NoBugs());
     }
 
     [TestMethod]
     [TestCategory("Manu")]
-    [Ignore] // Remove (or change test) once bug related to ref keyword is fixed
+    //[Ignore] // Remove (or change test) once bug related to ref keyword is fixed
     public void RefKeyword2()
     {
-        var corralResult = CorralTestHelper("RefKeyword", @"Test.RefKeyword.TestField$Test.RefKeyword", 10);
+        var corralResult = CorralTestHelper("RefKeyword", @"Test.RefKeyword.TestField$Test.RefKeyword", 10, useStubs: false, additionalTinyBCTOptions: "/NewAddrModelling=true");
         Assert.IsTrue(corralResult.NoBugs());
     }
 
@@ -2172,11 +2172,11 @@ class Test {
 
     // ************************************* DYNAMIC DISPATCH ******************************
 
-    [TestMethod, Timeout(10000)]
+    [TestMethod]
     [TestCategory("Manu")]
     public void DynamicDispatch1_NoBugs()
     {
-        var corralResult = CorralTestHelper("DynamicDispatch", @"DynamicDispatch.DynamicDispatch.test1_NoBugs", 10);
+        var corralResult = CorralTestHelper("DynamicDispatch", @"DynamicDispatch.DynamicDispatch.test1_NoBugs", 10, useStubs: false,  additionalTinyBCTOptions: "/NewAddrModelling=true");
         Assert.IsTrue(corralResult.NoBugs());
     }
 
