TinyBCT/Translators/MethodTranslator.cs
@@ -36,13 +36,13 @@ namespace TinyBCT
             var typeAnalysis = new TypeInferenceAnalysis(Traverser.CFG, methodBody.MethodDefinition.Type);
             typeAnalysis.Analyze();
 
-            /*var forwardCopyAnalysis = new ForwardCopyPropagationAnalysis(CFG);
+            var forwardCopyAnalysis = new ForwardCopyPropagationAnalysis(Traverser.CFG);
             forwardCopyAnalysis.Analyze();
             forwardCopyAnalysis.Transform(methodBody);
 
-            var backwardCopyAnalysis = new BackwardCopyPropagationAnalysis(CFG);
+            var backwardCopyAnalysis = new BackwardCopyPropagationAnalysis(Traverser.CFG);
             backwardCopyAnalysis.Analyze();
-            backwardCopyAnalysis.Transform(methodBody);*/
+            backwardCopyAnalysis.Transform(methodBody);
 
             // TinyBCT transformations
 
@@ -56,9 +56,8 @@ namespace TinyBCT
 
                 var fieldInitialization = new FieldInitialization(methodBody);
                 fieldInitialization.Transform();
-
-                methodBody.RemoveUnusedLabels();
             }
+            methodBody.RemoveUnusedLabels();
         }
 
 
@@ -131,7 +130,7 @@ namespace TinyBCT
             InstructionTranslator instTranslator = new InstructionTranslator(this.CHA, methodBody);
             instTranslator.Translate();
 
-            assignedInMethodCalls = instTranslator.AssignedInMethodCalls;
+            assignedInMethodCalls = instTranslator.ShouldCreateValueVariable;
 
             foreach (var v in instTranslator.RemovedVariables)
                 methodBody.Variables.Remove(v);
