TinyBCT/prelude.bpl
@@ -8,8 +8,9 @@ type Object = Union;
 var $AllocAddr: [Addr]bool;
 var $AllocObject: [Object]bool;
 
-//const unique null_addr: Addr;
-const unique null_object : Object;
+const unique null_addr: Addr;
+const null_object : Object;
+axiom null_object == null;
 
 type HeapInt = [Addr]int;
 type HeapBool = [Addr]bool;
@@ -26,11 +27,11 @@ procedure {:inline 1} AllocAddr() returns (x: Addr);
 implementation {:inline 1} AllocAddr() returns (x: Addr)
 {
     assume $AllocAddr[x] == false; //&& x != null_addr;
-	assume (forall aA : InstanceFieldAddr, oA : Object :: LoadInstanceFieldAddr(aA, oA) != x);
+	assume (forall aA : InstanceFieldAddr, oA : Object :: { LoadInstanceFieldAddr(aA, oA) } LoadInstanceFieldAddr(aA, oA) != x);
     $AllocAddr[x] := true;
 }
 
-axiom (forall aA, aB : InstanceFieldAddr, oA, oB : Object :: oA != oB ==> LoadInstanceFieldAddr(aA, oA) != LoadInstanceFieldAddr(aB, oB));
+axiom (forall aA, aB : InstanceFieldAddr, oA, oB : Object :: {LoadInstanceFieldAddr(aA, oA), LoadInstanceFieldAddr(aB, oB)} oA != oB ==> LoadInstanceFieldAddr(aA, oA) != LoadInstanceFieldAddr(aB, oB));
 
 procedure {:inline 1} AllocObject() returns (x: Object);
   modifies $AllocObject;
